src/Language/PlutusIR/Analysis/BoundVars/DecOpt.v
@@ -12,14 +12,14 @@ From QuickChick Require Import QuickChick.
 
 QCDerive DecOpt for (appears_bound_in_ty x ty).
 
-Instance appears_bound_in_ty_DecOpt_sound x ty: DecOptSoundPos (appears_bound_in_ty x ty).
-Proof. (* derive_sound. Qed. *) idtac "Admitted: appears_bound_in_ty_DecOpt_sound". Admitted.
+Instance DecOptappears_bound_in_ty_sound x ty: DecOptSoundPos (appears_bound_in_ty x ty).
+Proof. (* derive_sound. Qed. *) idtac "Admitted: DecOptappears_bound_in_ty_sound". Admitted.
 
-Instance appears_bound_in_ty_DecOpt_complete x ty: DecOptCompletePos (appears_bound_in_ty x ty).
-Proof. (* derive_complete. Qed. *) idtac "Admitted: appears_bound_in_ty_DecOpt_complete". Admitted.
+Instance DecOptappears_bound_in_ty_complete x ty: DecOptCompletePos (appears_bound_in_ty x ty).
+Proof. (* derive_complete. Qed. *) idtac "Admitted: DecOptappears_bound_in_ty_complete". Admitted.
 
-Instance appears_bound_in_ty_DecOpt_mono x ty: DecOptSizeMonotonic (appears_bound_in_ty x ty).
-Proof. (* derive_mon. Qed. *) idtac "Admitted: appears_bound_in_ty_DecOpt_mon". Admitted.
+Instance DecOptappears_bound_in_ty_mono x ty: DecOptSizeMonotonic (appears_bound_in_ty x ty).
+Proof. (* derive_mon. Qed. *) idtac "Admitted: DecOptappears_bound_in_ty_mon". Admitted.
 
 
 
@@ -27,25 +27,25 @@ Proof. (* derive_mon. Qed. *) idtac "Admitted: appears_bound_in_ty_DecOpt_mon". 
 
 QCDerive DecOpt for (appears_bound_in_tm x tm).
 
-Instance appears_bound_in_tm_DecOpt_sound x tm: DecOptSoundPos (appears_bound_in_tm x tm).
-Proof. (* derive_sound. Qed. *) idtac "Admitted: appears_bound_in_tm_DecOpt_sound". Admitted.
+Instance DecOptappears_bound_in_tm_sound x tm: DecOptSoundPos (appears_bound_in_tm x tm).
+Proof. (* derive_sound. Qed. *) idtac "Admitted: DecOptappears_bound_in_tm_sound". Admitted.
 
-Instance appears_bound_in_tm_DecOpt_complete x tm: DecOptCompletePos (appears_bound_in_tm x tm).
-Proof. (* derive_complete. Qed. *) idtac "Admitted: appears_bound_in_tm_DecOpt_complete". Admitted.
+Instance DecOptappears_bound_in_tm_complete x tm: DecOptCompletePos (appears_bound_in_tm x tm).
+Proof. (* derive_complete. Qed. *) idtac "Admitted: DecOptappears_bound_in_tm_complete". Admitted.
 
-Instance appears_bound_in_tm_DecOpt_mon x tm: DecOptSizeMonotonic (appears_bound_in_tm x tm).
-Proof. (* derive_mon. Qed. *) idtac "Admitted: appears_bound_in_tm_DecOpt_mon". Admitted.
+Instance DecOptappears_bound_in_tm_mon x tm: DecOptSizeMonotonic (appears_bound_in_tm x tm).
+Proof. (* derive_mon. Qed. *) idtac "Admitted: DecOptappears_bound_in_tm_mon". Admitted.
 
 
 (* appears_bound_in_ann *)
 
 QCDerive DecOpt for (appears_bound_in_ann x ann).
 
-Instance appears_bound_in_ann_DecOpt_sound x ann: DecOptSoundPos (appears_bound_in_ann x ann).
-Proof. (* derive_sound. Qed. *) idtac "Admitted: appears_bound_in_ann_DecOpt_sound". Admitted.
+Instance DecOptappears_bound_in_ann_sound x ann: DecOptSoundPos (appears_bound_in_ann x ann).
+Proof. (* derive_sound. Qed. *) idtac "Admitted: DecOptappears_bound_in_ann_sound". Admitted.
 
-Instance appears_bound_in_ann_DecOpt_complete x ann: DecOptCompletePos (appears_bound_in_ann x ann).
-Proof. (* derive_complete. Qed. *) idtac "Admitted: appears_bound_in_ann_DecOpt_complete". Admitted.
+Instance DecOptappears_bound_in_ann_complete x ann: DecOptCompletePos (appears_bound_in_ann x ann).
+Proof. (* derive_complete. Qed. *) idtac "Admitted: DecOptappears_bound_in_ann_complete". Admitted.
 
-Instance appears_bound_in_ann_DecOpt_mon x ann: DecOptSizeMonotonic (appears_bound_in_ann x ann).
-Proof. (* derive_mon. Qed. *) idtac "Admitted: appears_bound_in_ann_DecOpt_mon". Admitted.
+Instance DecOptappears_bound_in_ann_mon x ann: DecOptSizeMonotonic (appears_bound_in_ann x ann).
+Proof. (* derive_mon. Qed. *) idtac "Admitted: DecOptappears_bound_in_ann_mon". Admitted.
