src/Language/PlutusIR/Analysis/Purity/DecOpt.v
@@ -1,0 +1,32 @@
+From PlutusCert Require Import
+  Util.List
+  Util.DecOpt
+  Language.PlutusIR
+  Language.PlutusIR.DecOpt
+  Language.PlutusIR.Analysis.Purity
+  Language.PlutusIR.Semantics.Dynamic.Values
+  Language.PlutusIR.Semantics.Dynamic.Values.DecOpt.
+
+From QuickChick Require Import QuickChick.
+
+
+(* Used in the purity relation *)
+QCDerive EnumSized for binder_info.
+
+Instance Decbinder_info : Dec_Eq binder_info.
+Proof. dec_eq. Qed.
+
+
+
+QCDerive DecOpt for (is_pure Γ tm).
+
+Instance DecOptid_pure_sound Γ tm : DecOptSoundPos (is_pure Γ tm).
+Proof. derive_sound. Qed.
+
+
+
+
+QCDerive DecOpt for (pure_binding Γ tm).
+
+Instance DecOptpure_binding_sound Γ tm : DecOptSoundPos (pure_binding Γ tm).
+Proof. derive_sound. Qed.
