src/Language/PlutusIR/Analysis/UniqueBinders/DecOpt.v
@@ -11,8 +11,8 @@ From QuickChick Require Import QuickChick.
 
 QCDerive DecOpt for (unique_ty ty).
 
-Instance unique_ty_DecOpt_sound ty: DecOptSoundPos (unique_ty ty).
-Proof. (* derive_sound. Qed. *) idtac "Admitted: unique_ty_DecOpt_sound". Admitted.
+Instance DecOptunique_ty_sound ty: DecOptSoundPos (unique_ty ty).
+Proof. (* derive_sound. Qed. *) idtac "Admitted: DecOptunique_ty_sound". Admitted.
 
 (*
 Instance unique_ty_DecOpt_complete ty: DecOptCompletePos (unique_ty ty).
@@ -28,8 +28,8 @@ Proof. (* derive_mon. Qed. *) idtac "Admitted: unique_ty_DecOpt_mon". Admitted.
 
 QCDerive DecOpt for (unique_tm ty).
 
-Instance unique_tm_DecOpt_sound tm: DecOptSoundPos (unique_tm tm).
-Proof. (* derive_sound. Qed. *) idtac "Admitted: unique_tm_DecOpt_sound". Admitted.
+Instance DecOptunique_tm_sound tm: DecOptSoundPos (unique_tm tm).
+Proof. (* derive_sound. Qed. *) idtac "Admitted: DecOptunique_tm_sound". Admitted.
 
 (*
 Instance unique_tm_DecOpt_complete tm: DecOptCompletePos (unique_tm tm).
